finish proofs and clean up file structure

lean-circuit/Main.lean
@@ -5,148 +5,31 @@ import ProvenZk.Merkle
 import LeanCircuit
 import LeanCircuit.Poseidon.Spec
 import LeanCircuit.Poseidon.Correctness
+import LeanCircuit.SemanticEquivalence
 
-abbrev Order := Semaphore.Order
+open Semaphore (F Order)
+
 variable [Fact (Nat.Prime Order)]
-abbrev F := Semaphore.F
-
-def nat_to_dir : Nat -> Dir
-    | 0 => Dir.right
-    | 1 => Dir.left
-    | Nat.succ (Nat.succ _) => panic "Dir can be 0 or 1"
-
-def poseidon₁ : Hash F 1 := fun a => (Poseidon.perm Constants.x5_254_2 vec![0, a.get 0]).get 0
-def poseidon₂ : Hash F 2 := fun a => (Poseidon.perm Constants.x5_254_3 vec![0, a.get 0, a.get 1]).get 0
-
-def create_dir_vec {depth} (ix: Vector F depth) : Vector Dir depth :=
-    Vector.map nat_to_dir (Vector.map ZMod.val ix)
-
-abbrev secret (IdentityNullifier: F) (IdentityTrapdoor: F) : F :=
-    poseidon₂ vec![IdentityNullifier, IdentityTrapdoor]
-
-abbrev identity_commitment (IdentityNullifier: F) (IdentityTrapdoor: F) : F :=
-    poseidon₁ vec![(secret IdentityNullifier IdentityTrapdoor)]
-
-abbrev nullifier_hash (ExternalNullifier: F) (IdentityNullifier: F) : F :=
-    poseidon₂ vec![ExternalNullifier, IdentityNullifier]
-
-theorem same_hash_same_identity (IdentityNullifier₁ IdentityNullifier₂ IdentityTrapdoor₁ IdentityTrapdoor₂ : F)
-    [Fact (perfect_hash poseidon₂)]
-    [Fact (perfect_hash poseidon₁)]:
-    identity_commitment IdentityNullifier₁ IdentityTrapdoor₁ = identity_commitment IdentityNullifier₂ IdentityTrapdoor₂ ↔
-    (IdentityNullifier₁ = IdentityNullifier₂ ∧ IdentityTrapdoor₁ = IdentityTrapdoor₂) := by
-    apply Iff.intro
-    case mp => {
-        intro h
-        simp [Vector.eq_cons_iff] at h
-        assumption
-    }
-    case mpr => { intro h; simp [h] }
-
-def circuit_simpl (IdentityNullifier IdentityTrapdoor ExternalNullifier NullifierHash Root: F) (Path Proof: Vector F 3): Prop :=
-    NullifierHash = nullifier_hash ExternalNullifier IdentityNullifier ∧
-    MerkleTree.recover poseidon₂ (create_dir_vec Path) Proof (identity_commitment IdentityNullifier IdentityTrapdoor) = Root
-
--- def merkle_tree_recover_round (path : F) (node : F) (sibling : F) : F := match nat_to_dir path.val with
---     | Dir.left => poseidon₂ vec![node, sibling]
---     | Dir.right => poseidon₂ vec![sibling, node]
-
--- theorem merkle_recover_round_correct (Direction: F) (Hash: F) (Sibling: F) (k: F -> Prop) : 
---     Semaphore.MerkleTreeRecoverRound Direction Hash Sibling k = k (merkle_tree_recover_round Direction Hash Sibling) := by
---     sorry
-
-def merkle_tree_recover_rounds_cps (merkle_tree_recover_round : F -> F -> F -> (F -> Prop) -> Prop) (Leaf : F) (PathIndices Siblings : Vector F n) (k : F -> Prop) : Prop := match n with
-    | Nat.zero => k Leaf
-    | Nat.succ _ => 
-        merkle_tree_recover_round PathIndices.head Leaf Siblings.head fun next =>
-            merkle_tree_recover_rounds_cps merkle_tree_recover_round next PathIndices.tail Siblings.tail k
-
-theorem merkle_tree_recover_rounds_uncps
-    {Leaf : F}
-    {PathIndices Siblings : Vector F n}
-    {k : F -> Prop} 
-    {merkle_tree_recover_round_cps : F -> F -> F -> (F -> Prop) -> Prop}
-    -- {merkle_tree_recover_round_uncps : ∀ Leaf PathIndices Siblings k, merkle_tree_recover_round_cps Leaf PathIndices Siblings k = k (merkle_tree_recover_round Leaf PathIndices Siblings)}
-    : 
-    merkle_tree_recover_rounds_cps merkle_tree_recover_round_cps Leaf PathIndices Siblings k = k (MerkleTree.recover poseidon₂ (create_dir_vec PathIndices) Siblings Leaf) := by
-    induction n with
-    | zero => 
-        unfold merkle_tree_recover_rounds_cps
-        unfold MerkleTree.recover
-        rfl
-    | succ _ ih =>
-        unfold merkle_tree_recover_rounds_cps
-        simp [<-MerkleTree.recover_tail_reverse_equals_recover]
-        unfold MerkleTree.recover_tail
-        simp
-        
-        sorry
-
-def looped_merkle_tree_inclusion_proof (Leaf: F) (PathIndices: Vector F n) (Siblings: Vector F n) (k: F -> Prop): Prop :=
-    merkle_tree_recover_rounds_cps Semaphore.MerkleTreeRecoverRound Leaf PathIndices Siblings k
-
-theorem looped_merkle_tree_inclusion_proof_go (Leaf: F) (PathIndices: Vector F 3) (Siblings: Vector F 3) (k: F -> Prop):
-    Semaphore.MerkleTreeInclusionProof_3_3 Leaf PathIndices Siblings k = looped_merkle_tree_inclusion_proof Leaf PathIndices Siblings k := by
-    unfold Semaphore.MerkleTreeInclusionProof_3_3
-    unfold looped_merkle_tree_inclusion_proof
-    simp [merkle_tree_recover_rounds_cps]
-    simp [merkle_tree_recover_rounds_cps]
-    rw [←Vector.ofFn_get (v := PathIndices)]
-    rw [←Vector.ofFn_get (v := Siblings)]
-    rfl
-
-theorem merkle_tree_inclusion_proof_correct (Leaf: F) (PathIndices: Vector F 3) (Siblings: Vector F 3) (k: F -> Prop):
-  Semaphore.MerkleTreeInclusionProof_3_3 Leaf PathIndices Siblings k = k (MerkleTree.recover poseidon₂ (create_dir_vec PathIndices) Siblings Leaf) := by
-    simp [looped_merkle_tree_inclusion_proof_go]
-    simp [looped_merkle_tree_inclusion_proof]
-    simp [merkle_tree_recover_rounds_uncps]
-
-lemma circuit_simplified {IdentityNullifier IdentityTrapdoor SignalHash ExternalNullifier NullifierHash Root: F} {Path Proof: Vector F 3}:
-    Semaphore.circuit IdentityNullifier IdentityTrapdoor Path Proof SignalHash ExternalNullifier NullifierHash Root ↔
-    circuit_simpl IdentityNullifier IdentityTrapdoor ExternalNullifier NullifierHash Root Path Proof := by
-    simp [
-        Semaphore.circuit,
-        circuit_simpl,
-        Semaphore.Poseidon2,
-        Semaphore.Poseidon1,
-        nullifier_hash,
-        identity_commitment,
-        secret, poseidon₂,
-        poseidon₁,
-        Gates.eq,
-        poseidon_3_correct,
-        poseidon_2_correct,
-        merkle_tree_inclusion_proof_correct,
-        fold_vec_3
-    ]
-    apply Iff.intro <;> {
-        intro h
-        cases h
-        subst_vars
-        simp [getElem]
-        tauto
-    }
 
 theorem always_possible_to_signal
-    (IdentityNullifier IdentityTrapdoor SignalHash ExtNullifier : F)
-    (Tree : MerkleTree F poseidon₂ 3)
-    (Path : Vector F 3)
-    (comm_in_tree : Tree.item_at (create_dir_vec Path) = identity_commitment IdentityNullifier IdentityTrapdoor)
-    :
-    Semaphore.circuit
-        IdentityNullifier
-        IdentityTrapdoor
-        Path
-        (Tree.proof (create_dir_vec Path)) -- Siblings
-        SignalHash
-        ExtNullifier
-        (nullifier_hash ExtNullifier IdentityNullifier) -- NullifierHash
-        Tree.root := by
-        rw [circuit_simplified]
-        rw [←MerkleTree.recover_proof_is_root]
-        rw [comm_in_tree]
-        unfold circuit_simpl
-        simp
+  (IdentityNullifier IdentityTrapdoor SignalHash ExtNullifier : F)
+  (Tree : MerkleTree F poseidon₂ 3)
+  (Path : Vector Dir 3)
+  (commitment_in_tree : Tree.item_at Path = identity_commitment IdentityNullifier IdentityTrapdoor)
+  :
+  Semaphore.circuit
+    IdentityNullifier
+    IdentityTrapdoor
+    (embed_dir_vector Path.reverse)
+    (Tree.proof Path).reverse
+    SignalHash
+    ExtNullifier
+    (nullifier_hash ExtNullifier IdentityNullifier)
+    Tree.root
+  := by
+    rw [circuit_semantics, ←MerkleTree.recover_proof_is_root, commitment_in_tree]
+    simp [circuit_sem]
+    apply embed_dir_vector_is_binary
 
 theorem signaller_is_in_tree
     (IdentityNullifier IdentityTrapdoor SignalHash ExtNullifier NullifierHash : F)
@@ -155,12 +38,10 @@ theorem signaller_is_in_tree
     [Fact (perfect_hash poseidon₂)]
     :
     Semaphore.circuit IdentityNullifier IdentityTrapdoor Path Proof SignalHash ExtNullifier NullifierHash Tree.root →
-    Tree.item_at (create_dir_vec Path) = identity_commitment IdentityNullifier IdentityTrapdoor := by
-    rw [circuit_simplified]
-    intro h
-    unfold circuit_simpl at h
-    cases h
-    rw [<-MerkleTree.proof_ceritfies_item (create_dir_vec Path) Tree Proof (identity_commitment IdentityNullifier IdentityTrapdoor)]
+    Tree.item_at (create_dir_vec Path.reverse) = identity_commitment IdentityNullifier IdentityTrapdoor := by
+    simp [circuit_semantics, circuit_sem]
+    intros
+    apply MerkleTree.proof_ceritfies_item
     assumption
 
 theorem no_double_signal_with_same_commitment
@@ -174,10 +55,9 @@ theorem no_double_signal_with_same_commitment
     ExtNullifier₁ = ExtNullifier₂ →
     identity_commitment IdentityNullifier₁ IdentityTrapdoor₁ = identity_commitment IdentityNullifier₂ IdentityTrapdoor₂ →
     NullifierHash₁ = NullifierHash₂ := by
-    simp [circuit_simplified, circuit_simpl]
-    intro _ _ _ _ _ idCommEq
-    simp [secret, Vector.eq_cons_iff] at idCommEq
-    simp [*]
+    simp [circuit_semantics, circuit_sem, secret, Vector.eq_cons_iff]
+    intros
+    subst_vars
+    rfl
 
-def main : IO Unit := do
-    IO.println "Hello, world!"
+def main : IO Unit := pure ()
