lean-circuit/LeanCircuit/SemanticEquivalence.lean
@@ -1,0 +1,195 @@
+import ProvenZk.Binary
+import ProvenZk.Hash
+import ProvenZk.Merkle
+
+import LeanCircuit
+import LeanCircuit.Poseidon.Spec
+import LeanCircuit.Poseidon.Correctness
+
+open Semaphore (F Order)
+
+variable [Fact (Nat.Prime Order)]
+
+def nat_to_dir : Nat -> Dir
+  | 0 => Dir.left
+  | 1 => Dir.right
+  | Nat.succ (Nat.succ _) => panic "Dir can be 0 or 1"
+
+def create_dir_vec {depth} (ix: Vector F depth) : Vector Dir depth :=
+  Vector.map nat_to_dir (Vector.map ZMod.val ix)
+
+def embed_dir : Dir -> F
+  | Dir.left => 0
+  | Dir.right => 1
+
+def embed_dir_vector {depth} (ix: Vector Dir depth) : Vector F depth :=
+  Vector.map embed_dir ix
+
+lemma dir_embed_recover {d : Dir} : nat_to_dir (embed_dir d).val = d := by
+  cases d <;> rfl
+
+@[simp]
+lemma dir_embed_recover_vector {depth} (ix: Vector Dir depth) :
+  create_dir_vec (embed_dir_vector ix) = ix := by
+  simp [create_dir_vec, embed_dir_vector, dir_embed_recover]
+  apply Vector.eq
+  simp
+
+@[simp]
+lemma embed_dir_vector_reverse {depth} (ix : Vector Dir depth) :
+  embed_dir_vector ix.reverse = (embed_dir_vector ix).reverse := by
+  simp [embed_dir_vector]
+  apply Vector.eq
+  simp [Vector.toList_reverse, List.map_reverse]
+
+@[simp]
+lemma create_dir_vec_reverse {depth} (ix : Vector F depth) :
+  create_dir_vec ix.reverse = (create_dir_vec ix).reverse := by
+  simp [create_dir_vec]
+  apply Vector.eq
+  simp [Vector.toList_reverse, List.map_reverse]
+
+lemma foldr_snoc_cons {α β} {f : α -> β -> β} {b : β} {x : α} {xs : List α}
+  {f_comm_assoc : ∀ x y z, f x (f y z) = f y (f x z)} :
+  List.foldr f b (xs ++ [x]) = List.foldr f b (x :: xs) := by
+  induction xs generalizing x with
+  | nil => rfl
+  | cons x' xs ih =>
+    conv =>
+      lhs
+      simp only [List.foldr]
+      tactic => have : (xs ++ [x]) = xs.append [x] := by simp
+      rw [←this, ih]
+    simp [List.foldr, f_comm_assoc]
+
+lemma foldr_reverse {α β} {f : α -> β -> β} {b : β} {xs : List α}
+  { f_comm_assoc : ∀ x y z, f x (f y z) = f y (f x z) } :
+  List.foldr f b xs = List.foldr f b xs.reverse := by
+  induction xs with
+  | nil => rfl
+  | cons x xs ih =>
+    rw [List.reverse_cons, foldr_snoc_cons]
+    simp only [List.foldr, ih]
+    assumption
+
+@[simp]
+lemma is_vector_binary_reverse {depth} (ix : Vector F depth):
+  is_vector_binary ix.reverse ↔ is_vector_binary ix := by
+  simp only [is_vector_binary, Vector.toList_reverse]
+  rw [foldr_reverse]
+  { simp }
+  { intros; simp; tauto }
+
+lemma embed_dir_vector_is_binary {depth} (ix : Vector Dir depth) :
+  is_vector_binary (embed_dir_vector ix) := by
+  simp [is_vector_binary, embed_dir_vector]
+  induction ix using Vector.inductionOn with
+  | h_nil => simp [is_vector_binary]
+  | @h_cons n d ds ih =>
+    simp [is_vector_binary_cons]
+    apply And.intro
+    { simp [embed_dir, is_bit]; cases d <;> simp }
+    { assumption }
+
+def poseidon₁ : Hash F 1 := fun a => (Poseidon.perm Constants.x5_254_2 vec![0, a.get 0]).get 0
+
+lemma Poseidon1_uncps (a : F) (k : F -> Prop) : Semaphore.Poseidon1 a k ↔ k (poseidon₁ vec![a]) := by
+    simp [Semaphore.Poseidon1, poseidon₁, poseidon_2_correct, getElem]
+
+def poseidon₂ : Hash F 2 := fun a => (Poseidon.perm Constants.x5_254_3 vec![0, a.get 0, a.get 1]).get 0
+
+lemma Poseidon2_uncps (a b : F) (k : F -> Prop) : Semaphore.Poseidon2 a b k ↔ k (poseidon₂ vec![a, b]) := by
+    simp [Semaphore.Poseidon2, poseidon₂, poseidon_3_correct, getElem]
+    rfl
+
+@[simp]
+lemma create_dir_vec_cons {ix : F} {ixes: Vector F d} :
+  create_dir_vec (ix ::ᵥ ixes) = nat_to_dir ix.val ::ᵥ create_dir_vec ixes := by
+  simp [create_dir_vec]
+
+lemma MerkleTreeRecoverRound_uncps {dir hash sibling : F} {k : F -> Prop}:
+    Semaphore.MerkleTreeRecoverRound dir hash sibling k ↔
+    is_bit dir ∧ k (match nat_to_dir dir.val with
+    | Dir.left => poseidon₂ vec![hash, sibling]
+    | Dir.right => poseidon₂ vec![sibling, hash]) := by
+    simp [Semaphore.MerkleTreeRecoverRound, Gates.is_bool]
+    intro hb
+    rw [Poseidon2_uncps, Poseidon2_uncps]
+    cases hb <;> {
+        simp [*, Gates.select, Gates.is_bool, nat_to_dir]
+        try rfl
+    }
+
+def merkle_tree_recover_rounds (Leaf : F) (PathIndices Siblings : Vector F n) (k : F -> Prop) : Prop :=
+  match n with
+  | Nat.zero => k Leaf
+  | Nat.succ _ => Semaphore.MerkleTreeRecoverRound PathIndices.head Leaf Siblings.head fun next =>
+    merkle_tree_recover_rounds next PathIndices.tail Siblings.tail k
+
+lemma merkle_tree_recover_rounds_uncps
+  {Leaf : F}
+  {PathIndices Siblings : Vector F n}
+  {k : F -> Prop}:
+  merkle_tree_recover_rounds Leaf PathIndices Siblings k ↔
+  is_vector_binary PathIndices ∧ k (MerkleTree.recover_tail poseidon₂ (create_dir_vec PathIndices) Siblings Leaf) := by
+  induction PathIndices, Siblings using Vector.inductionOn₂ generalizing Leaf with
+  | nil =>
+    simp [is_vector_binary]
+    rfl
+  | @cons n ix sib ixes sibs ih =>
+    simp [MerkleTree.recover_tail_reverse_equals_recover, MerkleTree.recover_tail, merkle_tree_recover_rounds]
+    simp [MerkleTreeRecoverRound_uncps, is_vector_binary_cons, and_assoc, ih]
+    intros
+    rfl
+
+lemma MerkleTreeInclusionProof_looped (Leaf: F) (PathIndices: Vector F 3) (Siblings: Vector F 3) (k: F -> Prop):
+    Semaphore.MerkleTreeInclusionProof_3_3 Leaf PathIndices Siblings k =
+      merkle_tree_recover_rounds Leaf PathIndices Siblings k := by
+    unfold Semaphore.MerkleTreeInclusionProof_3_3
+    simp [merkle_tree_recover_rounds]
+    simp [merkle_tree_recover_rounds]
+    rw [←Vector.ofFn_get (v := PathIndices)]
+    rw [←Vector.ofFn_get (v := Siblings)]
+    rfl
+
+lemma MerkleTreeInclusionProof_3_3_uncps {Leaf : F} {PathIndices Siblings : Vector F 3} {k : F -> Prop}:
+    Semaphore.MerkleTreeInclusionProof_3_3 Leaf PathIndices Siblings k ↔
+    is_vector_binary PathIndices ∧ k (MerkleTree.recover_tail poseidon₂ (create_dir_vec PathIndices) Siblings Leaf) := by
+    simp [MerkleTreeInclusionProof_looped, merkle_tree_recover_rounds_uncps]
+
+abbrev secret (IdentityNullifier: F) (IdentityTrapdoor: F) : F :=
+  poseidon₂ vec![IdentityNullifier, IdentityTrapdoor]
+
+abbrev identity_commitment (IdentityNullifier: F) (IdentityTrapdoor: F) : F :=
+  poseidon₁ vec![(secret IdentityNullifier IdentityTrapdoor)]
+
+abbrev nullifier_hash (ExternalNullifier: F) (IdentityNullifier: F) : F :=
+  poseidon₂ vec![ExternalNullifier, IdentityNullifier]
+
+def circuit_sem (IdentityNullifier IdentityTrapdoor ExternalNullifier NullifierHash Root: F) (Path Proof: Vector F 3): Prop :=
+    NullifierHash = nullifier_hash ExternalNullifier IdentityNullifier ∧
+    is_vector_binary Path ∧
+    MerkleTree.recover poseidon₂ (create_dir_vec Path).reverse Proof.reverse (identity_commitment IdentityNullifier IdentityTrapdoor) = Root
+
+theorem circuit_semantics {IdentityNullifier IdentityTrapdoor SignalHash ExternalNullifier NullifierHash Root: F} {Path Proof: Vector F 3}:
+    Semaphore.circuit IdentityNullifier IdentityTrapdoor Path Proof SignalHash ExternalNullifier NullifierHash Root ↔
+    circuit_sem IdentityNullifier IdentityTrapdoor ExternalNullifier NullifierHash Root Path Proof := by
+    simp [
+      circuit_sem,
+      Semaphore.circuit,
+      Poseidon2_uncps,
+      Poseidon1_uncps,
+      MerkleTreeInclusionProof_3_3_uncps,
+      Gates.eq,
+      nullifier_hash,
+      create_dir_vec
+    ]
+    apply Iff.intro <;> {
+      intro h
+      cases h; rename_i _ r
+      cases r
+      subst_vars
+      rw [←Vector.ofFn_get (v := Path)] at *
+      rw [←Vector.ofFn_get (v := Proof)]
+      tauto
+    }
